Attempt at defining PRel

KLR/Semantics/SmallStep.lean
@@ -4,39 +4,175 @@ Released under Apache 2.0 license as described in the file LICENSE.
 Authors: Markus de Medeiros
 -/
 
+import Std.Data.HashMap
 
 /- # Mechanization of a generic nondeterministic small-step semantics -/
 
-class SmallStep (Pgm State Val : Type _) where
-  step : Pgm × State → Pgm × State → Prop
-  to_value : Pgm × State → Option Val
-  value_stuck : (to_value c).isSome → ¬∃ c', step c c'
+structure SmallStep : Type _ where
+  prog : Type _
+  state : Type _
+  val : Type _
+  step : prog × state → prog × state → Prop
+  to_val : prog × state → Option val
+  value_stuck {c c' : prog × state} : (to_val c).isSome → step c c' → False
 
-section SmallStep
+class SmallStepDet (S : SmallStep) where
+  step_det c : ∃ c', ∀ c'', S.step c c'' → c'' = c'
 
-variable (Pgm State Val : Type _) [I : SmallStep Pgm State Val]
+namespace SmallStep
 
-/-- A program can take exactly N steps between two states.
-This implies a trace where no intermediate state is a value, and is probably not useful. -/
-inductive stepExactN : Nat → Pgm × State → Pgm × State → Prop where
-| step0 : stepExactN 0 c c
-| stepS : SmallStep.step Val c c' → stepExactN n c' c'' → stepExactN n.succ c c''
+section basic
+variable (S : SmallStep)
 
-theorem stepExactN_1_iff_step : stepExactN Pgm State Val 1 (p, s) (p', s') ↔ I.step (p, s) (p', s') := by
-  refine ⟨?_, (stepExactN.stepS · stepExactN.step0)⟩
-  rintro (_|⟨_,_|_⟩)
-  trivial
+def stuck (c : S.prog × S.state) : Prop := ∀ c', ¬ S.step c c'
 
-theorem step_none (H : SmallStep.step Val (p2', s2') (p2, s2)) :
-    (SmallStep.to_value (Pgm := Pgm) (State := State) (Val := Val) (p2', s2')).isNone := by
-  suffices ¬(SmallStep.to_value (Val := Val) (p2', s2')).isSome by
-    generalize HX : (SmallStep.to_value (Val := Val) (p2', s2')) = X
-    rw [HX] at this
-    cases X <;> simp_all
-  intro H'
-  apply (SmallStep.value_stuck H')
-  exists (p2, s2)
+inductive stepN : Nat → S.prog × S.state → S.prog × S.state → Prop where
+| done : c = c' → stepN 0 c c'
+| step : S.step c c' → stepN n c' c'' → stepN n.succ c c''
 
+theorem stepN_zero_inv (H : S.stepN 0 c c') : c = c' := by cases H; trivial
+
+theorem stepN_stuck_inv (H : S.stepN m c c') (Hs : S.stuck c) : m = 0 := by
+  cases H
+  · rfl
+  · rename_i Hstep HstepN
+    exact (Hs _ Hstep).elim
+
+/-- For any of the first n steps of execution, all stuck states satisfy `Φ`. -/
+inductive satisfiesN (Φ : S.prog × S.state → Prop) : Nat → S.prog × S.state → Prop where
+| stuck : S.stuck c → Φ c → satisfiesN Φ n c
+| step  : S.step c c' → satisfiesN Φ n c' → satisfiesN Φ n.succ c
+
+/-
+theorem satisfiesN_stepN (H : S.satisfiesN Φ n c) : ∀ m, m ≤ n → S.stuck c' → S.stepN m c c' → Φ c' := by
+  revert c
+  induction n
+  · intro c H m Hm Hs Hs'
+    rw [Nat.le_zero_eq] at Hm
+    rcases H with ⟨_, H⟩
+    exact (stepN_zero_inv S (Hm▸Hs'))▸H
+  rename_i n IH
+  rintro c H m Hm Hstuck Hstep
+  cases H
+  · rename_i Hs' HΦ
+    have Hz := stepN_stuck_inv S Hstep Hs'
+    have Hc := stepN_zero_inv S (Hz ▸ Hstep)
+    exact Hc ▸ HΦ
+  rename_i _ Hsat Hstep'
+  rcases m with (_|m)
+  · exact Hstuck _ (stepN_zero_inv S Hstep ▸ Hstep') |>.elim
+  -- have Hm' := Nat.add_le_add_iff_right ▸ Hm
+  cases Hstep
+  -- apply IH Hsat _ (Nat.le_of_lt_succ Hm) Hstuck
+  sorry
+-/
+
+theorem stepN_1_iff_step : S.stepN 1 (p, s) (p', s') ↔ S.step (p, s) (p', s') := by
+  refine ⟨?_, (stepN.step · (stepN.done rfl))⟩
+  rintro (_|⟨H,He|_⟩)
+  exact He▸H
+
+theorem step_not_stuck (H : S.step (p1, s1) (p1', s1')) : (S.to_val (p1, s1)).isNone := by
+  have H' : ¬(S.to_val (p1, s1)).isSome → (S.to_val (p1, s1)).isNone := by
+    cases S.to_val (p1, s1) <;> simp
+  exact H' (S.value_stuck · H)
+
+end basic
+
+@[simp] abbrev prod.prog (S : SmallStep) := S.prog × S.prog
+@[simp] abbrev prod.state (S : SmallStep) := S.state × S.state
+@[simp] abbrev prod.val (S : SmallStep) := S.val × S.val
+
+inductive prod.step {S : SmallStep} : (prod.prog S) × (prod.state S) → (prod.prog S) × (prod.state S) → Prop where
+| step_l : S.step (p1, s1) (p1', s1') → prod.step ((p1, p2), (s1, s2)) ((p1, p2'), (s1, s2'))
+| step_r : S.step (p2, s2) (p2', s2') → prod.step ((p1, p2), (s1, s2)) ((p1, p2'), (s1, s2'))
+
+@[simp] def prod.to_val {S : SmallStep} (c : prod.prog S × prod.state S) : Option (prod.val S) :=
+  match S.to_val ⟨c.1.1, c.2.1⟩, S.to_val ⟨c.1.2, c.2.2⟩ with
+  | some v1, some v2 => some (v1, v2)
+  | _, _ => none
+
+theorem prod.value_stuck {S : SmallStep} {c c' : prod.prog S × prod.state S} :
+    (prod.to_val c).isSome → prod.step c c' → False := by
+  rcases c with ⟨⟨p1, p2⟩, ⟨s1, s2⟩⟩
+  simp only [to_val]
+  split
+  · rename_i Hv1 Hv2
+    intro _ Hstep; rcases Hstep with (Hs|Hs)
+    · exact S.value_stuck (Hv1▸rfl) Hs
+    · exact S.value_stuck (Hv2▸rfl) Hs
+  · simp
+
+def prod (S : SmallStep) : SmallStep where
+  prog := prod.prog S
+  state := prod.state S
+  val := prod.val S
+  step := prod.step
+  to_val := prod.to_val
+  value_stuck := prod.value_stuck
+
+/-
+
+-- There is a better way
+
+
+section prod
+
+variable {S : SmallStep}
+
+
+/-- Every n-step trace in the product semantics can be thought of as two traces in the semantics
+of the components. -/
+theorem prod.step_noninterference {n : Nat} :
+    S.prod.stepN n ((p, q), (s, t)) ((p', q'), (s', t')) ↔
+    (∃ mₗ mᵣ : Nat, n = mₗ + mᵣ ∧ S.stepN mₗ (p, s) (p', s') ∧ S.stepN mᵣ (q, t) (q', t')) :=
+  sorry
+
+def prod.π₁ (s : S.prod.prog × S.prod.state) : S.prog × S.state := ⟨s.1.1, s.2.1⟩
+def prod.π₂ (s : S.prod.prog × S.prod.state) : S.prog × S.state := ⟨s.1.2, s.2.2⟩
+def prod.mk (sₗ sᵣ : S.prog × S.state) : S.prod.prog × S.prod.state := ⟨⟨sₗ.1, sᵣ.1⟩, ⟨sₗ.2, sᵣ.2⟩⟩
+
+/-- Relational soundness of the product semantics: If every stuck product trace of at most (2n) steps
+satisfies Φ, then for every pair of stuck traces of at most n steps, the relation holds on their stuck values. -/
+theorem prod.satisfies_soundness_fin {n : Nat} :
+    S.prod.satisfiesN Φ (n + n) c →
+    ∀ mₗ mᵣ cₗ cᵣ,
+      mₗ < n → mᵣ < n →
+      S.stuck cₗ → S.stuck cᵣ →
+      S.stepN mₗ (prod.π₁ c) cₗ → S.stepN mₗ (prod.π₂ c) cᵣ →
+      Φ (prod.mk cₗ cᵣ) :=
+  sorry
+
+end prod
+-/
+
+
+/-- All traces of a configuration do not terminate. -/
+def nonterminating {S : SmallStep} (c : S.prog × S.state) : Prop :=
+  -- The program never gets stuck
+  ∀ n c', S.stepN n c c' → ¬ S.stuck c'
+
+/-- A conservative definition of program equivalence, which should work as long as our semantics
+is deterministic. -/
+def PRel {S : SmallStep}
+    (Φi : (S.prog × S.state) → (S.prog × S.state) → Prop)
+    (Φf : S.val → S.val → Prop) : Prop :=
+  -- For all starting configurations that are related by Φi,
+  ∀ c1 c2, Φi c1 c2 →
+  -- They are equiterminating,
+  (nonterminating c1 ↔ nonterminating c2) ∧
+  -- and for any two finite executions,
+  (∀ c1' c2' n m,
+    (S.stepN n c1 c1' ∧ S.stuck c1' ∧ S.stepN m c2 c2' ∧ S.stuck c2') →
+    -- They only ever get stuck in value states that are related by Φf
+    (∃ v1 v2, S.to_val c1' = some v1 ∧ S.to_val c2' = some v2 ∧ Φf v1 v2))
+
+
+
+namespace SmallStep
+
+
+/-
 theorem stepExactN_succ_some {n : Nat} (H : stepExactN Pgm State Val n.succ (p2', s2') (p2, s2)) :
     (SmallStep.to_value (Val := Val) (p2', s2')).isNone := by
   rcases H with (_|_)
@@ -48,16 +184,11 @@ theorem stepExactN_succ_some {n : Nat} (H : stepExactN Pgm State Val n.succ (p2'
   apply (SmallStep.value_stuck H)
   rename_i c _ _; exists c
 
-def stuck (c : Pgm × State) : Prop := ∀ c', ¬ SmallStep.step Val c c'
-
 /- A program terminates in a given configuration in at most n steps -/
 inductive stepTerm : Nat → Pgm × State → Pgm × State → Prop where
 | stepTerm_term : stuck Pgm State Val c → stepTerm n c c
 | stepTerm_run : SmallStep.step Val c c' → stepTerm n c' c'' → stepTerm n.succ c c''
 
-/-- For the first n steps of execution, all stuck states satisfy `Φ`. -/
-def satN (n : Nat) (Φ : Pgm × State → Prop) (c : Pgm × State) : Prop :=
-  ∀ c', stepTerm _ _ Val n c c' → Φ c'
 
 def is_value? (c : Pgm × State) : Prop := ¬ (SmallStep.to_value (Val := Val) c) = .none
 
@@ -77,48 +208,22 @@ def safeN (n : Nat) : Pgm × State → Prop :=
 def safe (c : Pgm × State) : Prop := ∀ n, safeN (I := I) _ _ _ n c
 
 end SmallStep
+-/
 
-
-section Product
-
-/- Lift a small-step semantics to product programs -/
-
-variable {Pgm State Val : Type _} [I : SmallStep Pgm State Val]
-
-/-- Stepping relation for product programs. -/
-inductive Product.step : (Pgm × Pgm) × State × State → (Pgm × Pgm) × State × State → Prop where
-| step_l : SmallStep.step Val (p1, s1) (p1', s1') → step ((p1, p2), (s1, s2)) ((p1, p2'), (s1, s2'))
-| step_r : SmallStep.step Val (p2, s2) (p2', s2') → step ((p1, p2), (s1, s2)) ((p1, p2'), (s1, s2'))
-
-def Product.to_value : (Pgm × Pgm) × State × State → Option (Val × Val)
-| ((p1, p2), (s1, s2)) =>
-  match I.to_value (p1, s1), I.to_value (p2, s2) with
-  | .some v1, .some v2 => .some (v1, v2)
-  | _, _ => .none
-
-instance Product.is_SmallStep : SmallStep (Pgm × Pgm) (State × State) (Val × Val) where
-  step := Product.step (I := I)
-  to_value := Product.to_value
-  value_stuck {c} := by
-    rcases c with ⟨⟨p1, p2⟩, ⟨s1, s2⟩⟩
-    simp only [to_value]
-    split
-    · rename_i v1 v2 Hv1 Hv2
-      intro _
-      rintro ⟨c, Hc⟩
-      cases Hc
-      · rename_i _ Hstep
-        have Hstep' := step_none Pgm State Val Hstep
-        simp [Hv1] at Hstep'
-      · rename_i _ Hstep
-        have Hstep' := step_none Pgm State Val Hstep
-        simp [Hv2] at Hstep'
-    · simp
-
+/-
 /-- Lift a relation on final values to a relation on program terms, which is trivially true for all non-value terms. -/
 def lift_rel (R : Val × State → Val × State → Prop) (p1 p2 : Pgm × State) : Prop :=
   match SmallStep.to_value p1, SmallStep.to_value p2 with
   | some v1, some v2 => R ⟨v1, p1.2⟩ ⟨v2, p2.2⟩
   | _, _ => True
 
+
+-- The product doesn't introduce "more nondeterminism" in for stuck executions.
+-- If we prove that a relational property holds for all at most (n+n)-step traces that end in stuck states,
+-- Then we know that for all traces of both left and right programs that take at most n steps that end in
+-- stuck states, their stuck states satisfy the relation R.
+-- The other direction does not hold, because the (n+n) steps don't have to by evenly divided between left
+-- steps and right steps.
+
 end Product
+-/
